prove transitity of mem_structure_eq

backend/CMinorExperiments.v
@@ -42,7 +42,7 @@ Section STMTINTERCHANGE.
   Definition s12: Cminor.stmt := Cminor.Sseq s1 s2.
   Definition s21: Cminor.stmt := Cminor.Sseq s2 s1.
 
-  Variable injf : Val.meminj.
+  Definition injf : meminj := Mem.flat_inj (Mem.nextblock ma).
   Variable begininj: Mem.inject injf ma mb.
 
 
@@ -53,9 +53,128 @@ Section STMTINTERCHANGE.
   Variable exec_s12: exec_stmt ge f sp  e ma s12 E0 e' ma' Out_normal.
   Variable exec_s21: exec_stmt ge f sp  e ma s21 E0 e' mb' Out_normal.
 
+  Record mem_structure_eq (f: meminj) (m1 m2: mem) :=
+    mk_mem_structure_eq {
+        mseq_perm:
+          forall b1 b2 delta ofs k p,
+            f b1 = Some(b2, delta) ->
+            Mem.perm m1 b1 ofs k p ->
+            Mem.perm m2 b2 (ofs + delta) k p;
+        mseq_align:
+          forall b1 b2 delta chunk ofs p,
+            f b1 = Some(b2, delta) ->
+            Mem.range_perm m1 b1 ofs (ofs + size_chunk chunk) Max p ->
+            (align_chunk chunk | delta);
+      }.
+
+  Lemma mem_inj_mem_structure_eq:
+    forall g m m',
+      Mem.mem_inj g m m' ->
+      mem_structure_eq g m m'.
+  Proof.
+    intros.
+    inversion H.
+    constructor; eassumption.
+  Qed.
+
+  Lemma mem_structure_eq_store:
+    forall f ge sp  e e' m m',
+    forall chunk addr a,
+      exec_stmt ge f sp e m
+                (Sstore chunk addr a)
+                E0 e' m' Out_normal ->
+      mem_structure_eq injf m m'.
+  Proof.
+    unfold injf.
+    intros until a.
+    intros execs.
+    inversion execs; subst.
+
+    rename H10 into store.
+    unfold Mem.storev in store.
+    destruct vaddr; try inversion store.
+
+
+    constructor.
+    - intros until p.
+      intros inj.
+      intros perm_m.
+
+      unfold Mem.flat_inj in inj.
+      destruct (plt b1 (Mem.nextblock ma)); inversion inj; subst.
+      replace (ofs + 0) with ofs.
+
+      eapply Mem.perm_store_1; try eassumption.
+      omega.
+    - intros until p.
+      intros inj.
+      intros range_perm_m.
+      
+      
+      unfold Mem.flat_inj in inj.
+      destruct (plt b1 (Mem.nextblock ma)); inversion inj; subst.
+
+      exists 0.
+      omega.
+  Qed.
+
+  Lemma mem_structure_eq_trans:
+    forall m1 m2 m3, mem_structure_eq injf m1 m2  ->
+                 mem_structure_eq injf m2 m3 ->
+                 mem_structure_eq injf m1 m3.
+  Proof.
+    intros until m3.
+    intros eq12 eq23.
+
+    inversion eq12.
+    inversion eq23.
+    
+    constructor.
+
+    - intros until p.
+      intros inj_b1.
+      intros perm.
+      eapply mseq_perm1.
+      eassumption.
+
+      replace ofs with (ofs + 0).
+      eapply mseq_perm0 with (b1 := b1).
+      unfold injf.
+      unfold Mem.flat_inj.
+      destruct (plt b1 (Mem.nextblock ma)).
+      reflexivity.
+      admit.
+      eassumption.
+      omega.
+
+    - intros until p.
+      intros inj_b1.
+      intros perm.
+      exists 0.
+      unfold injf in inj_b1.
+      unfold Mem.flat_inj in inj_b1.
+      destruct (plt b1 (Mem.nextblock ma)); inversion inj_b1; try omega.
+  Admitted.
+
+
+             
+
+
+
+
+
+
+
+      
+
+  
+
   Lemma meminj_new: Mem.mem_inj injf ma' mb'.
   Proof.
     constructor.
+    intros.
+
+    - (* permission *)
   Abort.
 
   Theorem flip_valid: Mem.inject injf ma' mb'.
